submission/SigGolfCandidate/Hypertree/KeygenLeafHeader.lean
@@ -47,7 +47,7 @@ def Code (image : Image) (p : Word) : Prop :=
   instructionAt image (p + 140) = some (.base (.ADDI .x11 .x11 768)) ∧
   instructionAt image (p + 144) = some (.base (.LUI .x12 128)) ∧
   instructionAt image (p + 148) = some (.base (.ADDI .x12 .x12 768)) ∧
-  instructionAt image (p + 152) = some (.base (.ADDI .x5 .x0 1))
+  instructionAt image (p + 152) = some (.base (.ADDI .x5 .x0 0))
 
 instance (image : Image) (p : Word) : Decidable (Code image p) :=
   inferInstanceAs (Decidable (_ ∧ _ ∧ _ ∧ _ ∧ _ ∧ _ ∧ _ ∧ _ ∧ _ ∧ _ ∧ _ ∧ _ ∧ _ ∧ _ ∧ _ ∧ _ ∧ _ ∧ _ ∧ _ ∧ _ ∧ _ ∧ _ ∧ _ ∧ _ ∧ _ ∧ _ ∧ _ ∧ _ ∧ _ ∧ _ ∧ _ ∧ _ ∧ _ ∧ _ ∧ _ ∧ _ ∧ _ ∧ _ ∧ _))
@@ -91,7 +91,7 @@ def state (s : MachineState) : MachineState :=
   let s := execInstrBr s (.ADDI .x11 .x11 768)
   let s := execInstrBr s (.LUI .x12 128)
   let s := execInstrBr s (.ADDI .x12 .x12 768)
-  execInstrBr s (.ADDI .x5 .x0 1)
+  execInstrBr s (.ADDI .x5 .x0 0)
 
 theorem block (image : Image) (p : Word) (code : Code image p)
     (s : MachineState) (pc : s.pc = p) : OrdinarySteps image s 39 (state s) := by
@@ -134,7 +134,7 @@ theorem block (image : Image) (p : Word) (code : Code image p)
   let s36 := execInstrBr s35 (.ADDI .x11 .x11 768)
   let s37 := execInstrBr s36 (.LUI .x12 128)
   let s38 := execInstrBr s37 (.ADDI .x12 .x12 768)
-  let s39 := execInstrBr s38 (.ADDI .x5 .x0 1)
+  let s39 := execInstrBr s38 (.ADDI .x5 .x0 0)
   apply OrdinarySteps.step s s1 _ (.base (.ADDI .x10 .x0 3)) 38
   · have hp : s.pc = p + 0 := by simp [execInstrBr, pc, BitVec.add_assoc]
     simpa only [fetch_at, hp] using c0
@@ -296,7 +296,7 @@ theorem block (image : Image) (p : Word) (code : Code image p)
   · have hp : s37.pc = p + 148 := by simp [s1, s2, s3, s4, s5, s6, s7, s8, s9, s10, s11, s12, s13, s14, s15, s16, s17, s18, s19, s20, s21, s22, s23, s24, s25, s26, s27, s28, s29, s30, s31, s32, s33, s34, s35, s36, s37, execInstrBr, pc, BitVec.add_assoc]
     simpa only [fetch_at, hp] using c37
   · rfl
-  apply OrdinarySteps.step s38 s39 _ (.base (.ADDI .x5 .x0 1)) 0
+  apply OrdinarySteps.step s38 s39 _ (.base (.ADDI .x5 .x0 0)) 0
   · have hp : s38.pc = p + 152 := by simp [s1, s2, s3, s4, s5, s6, s7, s8, s9, s10, s11, s12, s13, s14, s15, s16, s17, s18, s19, s20, s21, s22, s23, s24, s25, s26, s27, s28, s29, s30, s31, s32, s33, s34, s35, s36, s37, s38, execInstrBr, pc, BitVec.add_assoc]
     simpa only [fetch_at, hp] using c38
   · rfl
@@ -306,7 +306,7 @@ theorem pc (s : MachineState) : (state s).pc = s.pc + 156 := by
   simp [state,execInstrBr,BitVec.add_assoc]
 
 theorem regs (s : MachineState) :
-    (state s).getReg .x5 = 1 ∧ (state s).getReg .x10 = 0x80000 ∧
+    (state s).getReg .x5 = 0 ∧ (state s).getReg .x10 = 0x80000 ∧
     (state s).getReg .x11 = 768 ∧ (state s).getReg .x12 = 0x80300 := by
   simp [state,execInstrBr,signExtend12,MachineState.getReg_setReg_eq,MachineState.getReg_setReg_ne]
 
